TMeta/Elab/Lemmas.lean
@@ -1,0 +1,47 @@
+module
+
+namespace TMeta.Elab.Lemmas
+
+public section
+
+theorem pi_congr'
+    {α₁ α₂ : Sort u} {β₁ : α₁ → Sort v} (β₂ : α₂ → Sort v)
+    (hα : α₁ = α₂)
+    (hβ : ∀ x, β₁ x = β₂ (cast hα x)) :
+    ((x : α₁) → β₁ x) = ((x : α₂) → β₂ x) := by
+  subst hα
+  exact pi_congr hβ
+
+theorem app_hcongr
+    {α₁ α₂ : Sort u} {β₁ : α₁ → Sort v} (β₂ : α₂ → Sort v)
+    {f₁ : (x : α₁) → β₁ x} {f₂ : (x : α₂) → β₂ x}
+    {a₁ : α₁} {a₂ : α₂}
+    (hα : α₁ = α₂)
+    (hβ : ∀ x, β₁ x = β₂ (cast hα x))
+    (hf : cast (pi_congr' β₂ hα hβ) f₁ = f₂)
+    (ha : cast hα a₁ = a₂) :
+    f₁ a₁ ≍ f₂ a₂ := by
+  subst hα
+  subst a₂
+  have hβ' : β₁ = β₂ := funext hβ
+  subst hβ'
+  rw [cast_eq] at hf
+  subst f₂
+  rfl
+
+theorem hfunext
+    {α₁ α₂ : Sort u} {β₁ : α₁ → Sort v} (β₂ : α₂ → Sort v)
+    {f₁ : (x : α₁) → β₁ x} (f₂ : (x : α₂) → β₂ x)
+    (hα : α₁ = α₂)
+    (h : ∀ x, f₁ x ≍ f₂ (cast hα x)) :
+    f₁ ≍ f₂ := by
+  subst hα
+  have hβ : β₁ = β₂ := funext fun x => type_eq_of_heq (h x)
+  subst hβ
+  apply heq_of_eq
+  funext x
+  exact eq_of_heq (h x)
+
+end
+
+end TMeta.Elab.Lemmas
